src/program_proof/simplepb/pb_roapply_proof.v
@@ -18,12 +18,14 @@ Context {pb_record:Sm.t}.
 Notation OpType := (Sm.OpType pb_record).
 Notation has_op_encoding := (Sm.has_op_encoding pb_record).
 Notation compute_reply := (Sm.compute_reply pb_record).
+Notation is_readonly_op := (Sm.is_readonly_op pb_record).
 Notation pbG := (pbG (pb_record:=pb_record)).
 
 Context `{!pbG Σ}.
 
 Lemma wp_Clerk__ApplyRo γ γsrv ck op_sl q op (op_bytes:list u8) (Φ:val → iProp Σ) :
 has_op_encoding op_bytes op →
+is_readonly_op op →
 is_Clerk ck γ γsrv -∗
 is_slice_small op_sl byteT q op_bytes -∗
 □((|={⊤∖↑pbN,∅}=> ∃ ops, own_int_log γ ops ∗
@@ -36,7 +38,7 @@ is_slice_small op_sl byteT q op_bytes -∗
                                      Φ (#err, (slice_val unused_sl))%V )) -∗
 WP Clerk__ApplyRo #ck (slice_val op_sl) {{ Φ }}.
 Proof.
-  intros Henc.
+  intros Henc Hro.
   iIntros "#Hck Hop_sl".
   iIntros "#HΦ".
   wp_call.
@@ -57,6 +59,7 @@ Proof.
     iNext.
     unfold Apply_spec.
     iExists _.
+    iSplitR; first done.
     iSplitR; first done.
     iSplit.
     {
@@ -149,14 +152,14 @@ Proof.
   naive_solver.
 Qed.
 
-Lemma generate_read_fupd γ Φ :
+Lemma generate_read_fupd γ Φ rop :
   is_inv γ -∗
   (|={⊤ ∖ ↑pbN,∅}=>
     ∃ ops, own_int_log γ ops ∗
-      (own_int_log γ ops ={∅,⊤ ∖ ↑pbN}=∗ □ Φ ops)) -∗
+      (own_int_log γ ops ={∅,⊤ ∖ ↑pbN}=∗ □ Φ (compute_reply ops rop))) -∗
   (|={⊤ ∖ ↑pbN ∪ ↑appN,∅}=>
     ∃ σ, own_pre_log γ.(s_prelog) σ ∗
-      (own_pre_log γ.(s_prelog) σ ={∅,⊤ ∖ ↑pbN ∪ ↑appN}=∗ □ Φ σ.*1))
+      (own_pre_log γ.(s_prelog) σ ={∅,⊤ ∖ ↑pbN ∪ ↑appN}=∗ □ Φ (compute_reply (get_rwops σ) rop)))
 .
 Proof.
   iIntros "#Hinv Hupd".
@@ -171,8 +174,8 @@ Proof.
   iExists _; iFrame.
   iIntros "Hghost".
   iMod ("Hupd" with "Hlog2") as "#Hupd".
-  rewrite -H.
   unfold get_rwops.
+  rewrite -H.
   iFrame "#".
   iMod "Hmask".
   iMod ("Hclose" with "[-]"); last done.
@@ -183,16 +186,18 @@ Proof.
   iExists _; iFrame "∗#%".
 Qed.
 
-Lemma preread_step st γ γsrv t Q {own_StateMachine} :
+Lemma preread_step st γ γsrv t (lastModifiedIndex:u64) Q rop {own_StateMachine} :
   st.(server.leaseValid) = true →
   int.nat t < int.nat st.(server.leaseExpiration) →
+  (∀ σ', prefix σ' st.(server.ops_full_eph) →
+         int.nat lastModifiedIndex <= length σ' → compute_reply (get_rwops σ') rop = compute_reply (get_rwops st.(server.ops_full_eph)) rop) →
   £ 1 -∗
   £ 1 -∗
   £ 1 -∗
   own_time t -∗
   □(|={⊤ ∖ ↑pbN ∪ ↑appN,∅}=>
     ∃ σ, own_pre_log γ.(s_prelog) σ ∗
-      (own_pre_log γ.(s_prelog) σ ={∅,⊤ ∖ ↑pbN ∪ ↑appN}=∗ □ Q σ)) -∗
+      (own_pre_log γ.(s_prelog) σ ={∅,⊤ ∖ ↑pbN ∪ ↑appN}=∗ □ Q (compute_reply (get_rwops σ) rop))) -∗
   own_Server_ghost_eph_f st γ γsrv -∗
   accessP_fact own_StateMachine (own_Server_ghost_f γ γsrv) -∗
   own_StateMachine st.(server.epoch) (get_rwops st.(server.ops_full_eph)) st.(server.sealed) (own_Server_ghost_f γ γsrv) -∗
@@ -200,12 +205,12 @@ Lemma preread_step st γ γsrv t Q {own_StateMachine} :
   |NC={⊤}=>
   own_StateMachine st.(server.epoch) (get_rwops st.(server.ops_full_eph)) st.(server.sealed) (own_Server_ghost_f γ γsrv) ∗
   preread_inv γ.(s_pb) γ.(s_prelog) γ.(s_reads) ∗
-  is_proposed_read γ.(s_reads) (length st.(server.ops_full_eph)) Q ∗
+  is_proposed_read γ.(s_reads) (int.nat lastModifiedIndex) (λ σ, Q (compute_reply (get_rwops σ) rop)) ∗
   is_proposal_lb γ.(s_pb) st.(server.epoch) st.(server.ops_full_eph) ∗
   own_time t ∗
   own_Server_ghost_eph_f st γ γsrv.
 Proof.
-  iIntros (??) "Hlc Hlc2 Hlc3 Htime #Hupd Hghost #HaccP Hstate #HpbInv".
+  iIntros (?? HlastModified) "Hlc Hlc2 Hlc3 Htime #Hupd Hghost #HaccP Hstate #HpbInv".
   iEval (rewrite /own_Server_ghost_eph_f /tc_opaque) in "Hghost".
   iNamed "Hghost".
   iNamed "Hlease".
@@ -287,9 +292,20 @@ Proof.
     }
   }
 
-  iMod (start_read_step with "Hlc2 [$] [Hupd] Hcommit") as "[$ Hcommit]".
+  iMod (start_read_step _ _ _ _ lastModifiedIndex (λ someσ, compute_reply (get_rwops someσ) rop)
+         with "Hlc2 [$] [Hupd] Hcommit") as "[H Hcommit]".
   { solve_ndisj. }
-  { by apply prefix_length. }
+  { intros.
+    epose proof (HlastModified σ _ _) as ->.
+    epose proof (HlastModified σ' _ _) as ->.
+    done.
+    Unshelve.
+    2:{ etransitivity; done. }
+    2:{ apply prefix_length in H3. word. }
+    2:{ by etransitivity. }
+    2:{ word. }
+    shelve.
+  }
   {
     iModIntro.
     iMod (fupd_mask_subseteq (⊤∖↑pbN ∪ ↑appN)) as "Hmask".
@@ -304,6 +320,7 @@ Proof.
     iIntros "?". iMod ("Hupd" with "[$]").
     by iMod "Hmask".
   }
+  iFrame "H".
   iMod ("HclosePb" with "[-Htime Hprimary Hghost Hprim_escrow]").
   { iNext; repeat iExists _; iFrame "∗#". }
   iModIntro.
@@ -376,7 +393,7 @@ Proof.
   iIntros "#Hsrv #Hop_sl".
   iIntros "HΨ HΦ".
   iApply (wp_frame_wand with "HΨ").
-  iDestruct "HΦ" as "(%Hop_enc & #Hupd & #Hfail_Φ)".
+  iDestruct "HΦ" as "(%Hop_enc & %Hro & #Hupd & #Hfail_Φ)".
   iNamed "Hsrv".
   rewrite /Server__ApplyRoWaitForCommit.
   wp_pure1_credit "Hlc1".
@@ -421,6 +438,23 @@ Proof.
     }
     by iApply "Hfail_Φ".
   }
+
+  wp_apply wp_ref_of_zero.
+  { done. }
+  iIntros (lastModified) "HlastModified".
+  wp_pures.
+  iDestruct (is_StateMachine_acc_applyReadonly with "HisSm") as "H".
+  iNamed "H".
+  wp_loadField.
+  wp_loadField.
+  wp_apply ("HapplySpec" with "[$Hstate]").
+  { iFrame "#%". }
+  iIntros (???) "(%HlastModifiedLen & %HlastModified & Hrep_sl & Hstate)".
+  wp_pures.
+  wp_store.
+  wp_storeField.
+  wp_loadField.
+
   wp_apply wp_GetTimeRange.
   iIntros (?????) "Htime".
   destruct (decide (int.nat h < int.nat st.(server.leaseExpiration))).
@@ -431,16 +465,24 @@ Proof.
        a
        Combine with
      *)
-    iMod (preread_step with "Hlc1 Hlc2 Hlc3 Htime [] HghostEph [] [Hstate] [$]") as "HH".
+    iMod (preread_step _ _ _ _ lastModifiedIndex with "Hlc1 Hlc2 Hlc3 Htime [] HghostEph [] [Hstate] [$]") as "HH".
     { done. }
     { word. }
-    {
-      iModIntro.
-      iApply generate_read_fupd.
+    { intros.
+      epose proof (HlastModified _ _) as ->.
+      1: done.
+      by rewrite fmap_length.
+    }
+    { iModIntro. iApply generate_read_fupd.
       { iFrame "#". }
-      { iFrame "#". }
+      {
+        instantiate (1:=(λ b,
+                          Ψ {| ApplyReply.err := 0; ApplyReply.ret := b |})
+                    ).
+        iFrame "#". }
     }
     {
+      iClear "Happly HapplySpec".
       rewrite /is_StateMachine /tc_opaque.
       by iNamed "HisSm".
     }
@@ -452,22 +494,9 @@ Proof.
     wp_loadField.
     wp_if_destruct.
     { exfalso. word. }
-    wp_loadField.
-    iDestruct (is_StateMachine_acc_applyReadonly with "HisSm") as "H".
-    iNamed "H".
-    wp_loadField.
-    wp_apply ("HapplySpec" with "[$Hstate]").
-    {
-      iSplitL; first done.
-      iFrame "#".
-    }
-    iIntros (??) "[Hrep_sl Hstate]".
-    wp_storeField.
-    wp_loadField.
-    wp_loadField.
     wp_pures.
 
-    iAssert (mu_inv s γ γsrv mu) with "[-Err Reply Hlocked Hrep_sl]" as "Hown".
+    iAssert (mu_inv s γ γsrv mu) with "[-Err Reply Hlocked Hrep_sl HlastModified]" as "Hown".
     {
       repeat iExists _; iSplitR "HghostEph"; last by iFrame.
       repeat iExists _; iFrame "∗#%".
@@ -502,6 +531,7 @@ Proof.
       }
       by iApply "Hfail_Φ".
     }
+    wp_load.
     wp_loadField.
     wp_pure1_credit "Hlc2".
     wp_pures.
@@ -509,10 +539,19 @@ Proof.
     { (* the read is finished! *)
       wp_storeField.
       iRight.
-      iMod (roapply_finish_step with "Hlc Hlc2 [] Hprop_read [$] HghostEph") as "H".
+      iMod (roapply_finish_step _ _ _ _ (take (int.nat lastModifiedIndex) st.(server.ops_full_eph))
+             with "Hlc Hlc2 [] [Hprop_read] [] HghostEph") as "H".
       { rewrite fmap_length /no_overflow in Heqb2 HnextIndexNoOverflow.
-        word. }
-      { rewrite -Heqb1. iFrame "Hprop_lb". }
+        rewrite take_length. word. }
+      { rewrite -Heqb1. iDestruct (fmlist_ptsto_lb_mono with "Hprop_lb") as "$".
+        eexists (drop _ _). by setoid_rewrite take_drop.
+      }
+      {
+        rewrite take_length_le; first iFrame "#".
+        rewrite fmap_length in HlastModifiedLen.
+        word.
+      }
+      { iFrame "#". }
       iDestruct "H" as "[HghostEph HΨ]".
       iModIntro. iSplitR; first done.
       wp_pures.
@@ -529,11 +568,31 @@ Proof.
       iIntros "HΦ".
       iApply ("HΦ" with "[$]").
       repeat iExists _; iFrame.
+      simpl.
+      iApply to_named.
+      iExactEq "Hrep_sl".
+      f_equal.
+      epose proof (HlastModified _ _) as ->.
+      { done. }
+      { rewrite fmap_length.
+        rewrite take_length_le.
+        1: done.
+        { rewrite fmap_length in HlastModifiedLen. word. }
+      }
+      Unshelve.
+      { destruct H1 as [? ?].
+        exists (get_rwops x). rewrite -fmap_app. unfold get_rwops.
+        by rewrite H1.
+      }
+      {
+        exists (get_rwops (drop (int.nat lastModifiedIndex) st.(server.ops_full_eph))).
+        rewrite -fmap_app. rewrite take_drop. done.
+      }
     }
     wp_loadField.
     iClear "HopAppliedConds_conds HcommittedNextIndex_is_cond".
     iNamed "Hvol".
-    wp_apply (wp_condWait with "[-Err Reply Hrep_sl]").
+    wp_apply (wp_condWait with "[-Err Reply Hrep_sl HlastModified]").
     {
       iFrame "#".
       iFrame "Hlocked".
@@ -555,7 +614,7 @@ Proof.
     wp_if_destruct.
     2:{ exfalso. word. }
     wp_loadField.
-    wp_apply (release_spec with "[-Err Reply]").
+    wp_apply (release_spec with "[-Err Reply HlastModified Hrep_sl]").
     {
       iFrame "HmuInv Hlocked".
       iNext.
@@ -568,8 +627,7 @@ Proof.
     iIntros "HΦ".
     iApply ("HΦ" $! (ApplyReply.mkC _ _)).
     2:{
-      iExists _, 1%Qp. iFrame.
-      by iApply is_slice_small_nil.
+      iExists _, _. iFrame.
     }
     { by iApply "Hfail_Φ". }
   }
